ocaml/debruijn.ml
@@ -64,7 +64,8 @@ let convert_fn_def (f : named_fn_def) : fn_def =
       (sc', acc @ [p]))
     ([], []) f.nf_params
   in
-  { fn_name   = make_ident f.nf_name 0;
-    fn_params = params;
-    fn_ret    = f.nf_ret;
-    fn_body   = convert scope f.nf_body }
+  { fn_name      = make_ident f.nf_name 0;
+    fn_lifetimes = Big_int_Z.big_int_of_int (List.length f.nf_lifetime_names);
+    fn_params    = params;
+    fn_ret       = f.nf_ret;
+    fn_body      = convert scope f.nf_body }
